Cleanup, getting close to handoff

model/isabelle/BW2.thy
@@ -5,22 +5,20 @@ imports "Carry_Val"
 begin
 
 text \<open>
-Upgrade of the existing Word_Bitwise conversion to booleans.
+Rework of the previous Word_Bitwise conversion to booleans.
 
-The main change is, the whole mechanism now permits sharing of
-repeated terms using let bindings. Values of word type may be
-let bound in input problems. The core tactic produces let
-bindings of shared boolean values. A final step can discard
-them (compatibility with previous version) or lift them to
-fresh meta-bound variables. The latter form seems to be quite
-compatible with the Argo solver.
+The mechanism shares repeated terms using let-bindings and
+then equalities. Values of word type may be let bound in input
+problems and will not be repeated in the output.
+
+The previous strategy of iterating over lists is dropped.
+Instead the @{const bit} constant is expanded by using its
+named theorem set.
+
+Ripple/carry effects are managed via the @{const carry_val} carry constant.
 \<close>
 
-lemma word_if_add_let:
-  "(if P then (x :: ('a :: len0) word) else y) = (let switch = P in id If switch x y)"
-  by simp
-
-lemmas bit_if = if_distrib[where f="\<lambda>x. bit x _"]
+lemmas bit_if[bit_simps] = if_distrib[where f="\<lambda>x. bit x _"]
 
 lemma bit_unat:
   "bit (unat (w :: ('a :: len) word)) i = bit w i"
@@ -37,10 +35,6 @@ lemma bit_word_numeral_eq_nat:
 lemma bit_word_numeral_eq_int:
   "bit (numeral n :: ('a :: len) word) i = bit (take_bit (LENGTH('a)) (numeral n :: int)) i"
   by (simp only: bit_uint[symmetric] uint_bintrunc)
-
-lemma bit_use_drop_bit:
-  "j \<le> i \<Longrightarrow> bit x i = bit (drop_bit j x) (i - j)"
-  by (simp add: bit_simps)
 
 ML \<open>
 structure Let_Alt = struct
@@ -63,21 +57,16 @@ fun simproc count ct = case strip_comb (Thm.term_of ct) of
   | (_, [_, _]) => SOME def
   | _ => NONE
 
-fun has_bv (Bound _) = true
-  | has_bv (Abs _) = true
-  | has_bv (f $ x) = has_bv f orelse has_bv x
-  | has_bv _ = false
-
-fun count_no_bv pred (t :: ts) tab = let
+fun count_subterms pred (t :: ts) tab = let
     val ts = case t of
         f $ x => f :: x :: ts
       | Abs (_, _, t) => t :: ts
       | _ => ts
-    val tab = if has_bv t then tab
-        else if pred t then Termtab.map_default (t, 0) (fn i => i + 1) tab
+    val tab = if pred t andalso null (loose_bnos t)
+        then Termtab.map_default (t, 0) (fn i => i + 1) tab
         else tab
-  in count_no_bv pred ts tab end
-  | count_no_bv _ [] tab = tab
+  in count_subterms pred ts tab end
+  | count_subterms _ [] tab = tab
 
 val sym_def = @{thm Let_def[symmetric]}
 
@@ -86,18 +75,15 @@ fun add_let_conv ctxt nm x ct = let
   in Drule.infer_instantiate ctxt [(("f", 0), abs), (("s", 0), x)] sym_def end
 
 fun let_gather_dup_conv_1 ctxt f ct = let
-    val count = count_no_bv f [Thm.term_of ct] Termtab.empty
+    val count = count_subterms f [Thm.term_of ct] Termtab.empty
     val xs = Termtab.dest count
       |> filter (fn (_, j) => j >= 2)
-      |> map fst
-      |> filter (not o is_atom)
-    fun get_greatest [] t _ = t
-      | get_greatest (x :: xs) t sz = if size_of_term x > sz
-        then get_greatest xs x (size_of_term x)
-        else get_greatest xs t sz
-    fun get_greatest2 xs = get_greatest (tl xs) (hd xs) (size_of_term (hd xs))
+      |> filter (not o is_atom o fst)
+      |> map (fn (t, _) => (size_of_term t, t))
+      |> sort (Int.compare o apply2 fst)
+      |> rev
   in if null xs then Conv.no_conv ct
-    else add_let_conv ctxt "x" (Thm.cterm_of ctxt (get_greatest2 xs)) ct
+    else add_let_conv ctxt "x" (Thm.cterm_of ctxt (snd (hd xs))) ct
   end
 
 fun let_gather_dup_conv ctxt f = Conv.repeat_conv (let_gather_dup_conv_1 ctxt f)
@@ -150,7 +136,7 @@ simproc_setup let_atom ("Let v f") = \<open>K (K (Let_Alt.simproc false))\<close
 declare [[simproc del: let_atom]]
 
 lemma let_eq_impI:
-  "(\<And>x. v = x \<Longrightarrow> P x) \<Longrightarrow> let x = v in P x"
+  "(\<And>x. v = x \<longrightarrow> P x) \<Longrightarrow> let x = v in P x"
   by simp
 
 lemmas carry_let_eq_impI = let_eq_impI[where v="carry_val x y c", unfolded carry_val_word_eq_eq]
@@ -159,15 +145,14 @@ lemmas carry_let_eq_impI = let_eq_impI[where v="carry_val x y c", unfolded carry
 lemmas word_let_eq_impI = let_eq_impI[where v=x, unfolded word_bit_eq_iff]
   for x :: "('a :: len) word"
 
-lemma case_nat_eq_If:
-  "(case n of 0 \<Rightarrow> x | Suc i \<Rightarrow> f i) = (if n = 0 then x else f (n - 1))"
-  by (cases n, auto)
+lemma ball_set_simps:
+  "(\<forall>x \<in> set (y # ys). P x) = (P y \<and> (\<forall>x \<in> set ys. P x))"
+  "(\<forall>x \<in> set []. P x) = True"
+  by simp_all
 
-lemma ball_insert:
-  "(\<forall>x \<in> insert y S. P x) = (P y \<and> (\<forall>x \<in> S. P x))"
+lemma imp_to_id:
+  "(P \<longrightarrow> Q) = id (\<longrightarrow>) P Q"
   by simp
-
-lemmas imp_to_id = id_apply[where x="(\<longrightarrow>)", THEN fun_cong, THEN fun_cong, symmetric]
 
 lemma bit_num_0[bit_simps]:
   "\<not> bit 0 x"
@@ -177,6 +162,7 @@ lemmas if_simps = if_bool_eq_disj[where Q=False, simplified]
   if_bool_eq_disj[where R=False, simplified]
   if_bool_eq_conj[where Q=True, simplified]
   if_bool_eq_conj[where R=True, simplified]
+  if_True if_False
 
 lemma carry_simps:
   "carry True a b = (a \<or> b)"
@@ -186,6 +172,11 @@ lemma carry_simps:
   "carry a False b = (a \<and> b)"
   "carry a b False = (a \<and> b)"
   by (auto simp add: carry_def)
+
+lemma bit_word_impossible:
+  fixes x :: "('a :: len) word"
+  shows "LENGTH ('a) \<le> i \<Longrightarrow> \<not> bit x i"
+  by (auto dest: bit_imp_le_length)
 
 ML \<open>
 structure Mk_Cache_Simproc = struct
@@ -208,36 +199,19 @@ ML \<open>
 structure BW_Alt = struct
 
 (* strategy:
-  1) rewrite with word_via_carry_val and word_if_add_let introducing lets
-  (init_tac)
-  2a) lift lets to top of goal and then to assumptions (let_eq_impI)
-    - also convert carry equals and other word equals to bitwise eqs
-  2b) pull assumptions with "bit" or "test_bit" back into the goal
-  (let_tac)
-  3a) hide implications from the simplifier (imp_to_id)
-      and unfold remaining word eqs to bitwise
-  3b) simplify with:
+  1) asm_tac (optional): rewrite equalities/inequalities to include bit
+    judgements, and pull all assumptions containing the bit constant into
+    the goal.
+  2) let_tac: rewrite word arithmetic to use the carry val,
+    then lift out carry values, values fixed in lets, and switches of if
+    terms up to top-level lets then assumptions
+  3) main_tac: first hide implications from the simplifier, then
+    do the main simplification phase:
+    - bit rewrites (bit_simps)
     - caching simproc for natural arithmetic and word lengths
-    - upt/ball rules
-    - bit substitutions
-    - exp_eq_zero_iff from Word (2 ^ n = 0 \<longrightarrow> ineq)
-  3c) restore implications
-  (main_tac)
+    - upt/ball expansion rules
+    - exponent rule from Word (2-to-the-power-of-n = 0 to ineq)
 *)
-
-val no_split_ss =
-  simpset_of (put_simpset HOL_ss \<^context>
-        delsimprocs [@{simproc let_simp}]
-        delsimps @{thms subst_all}
-    |> Splitter.del_split @{thm if_split});
-
-val init_ss = simpset_of (put_simpset HOL_basic_ss \<^context> addsimps
-   @{thms word_via_carry_val word_if_add_let})
-
-fun init_tac ctxt = simp_tac (put_simpset init_ss ctxt)
-    THEN_ALL_NEW simp_tac (put_simpset HOL_basic_ss ctxt addsimps @{thms id_apply})
-
-val is_word = can Word_Lib.dest_wordT o fastype_of
 
 fun rev_mp_prems_step_tac pred ctxt = DETERM o SUBGOAL (fn (t, i) => let
     val prems = Logic.strip_assums_hyp t
@@ -249,15 +223,57 @@ fun rev_mp_prems_step_tac pred ctxt = DETERM o SUBGOAL (fn (t, i) => let
 
 fun rev_mp_prems_tac pred ctxt = REPEAT_DETERM o (rev_mp_prems_step_tac pred ctxt)
 
-fun let_to_imp_step ctxt = FIRST'
-  [CHANGED o Let_Alt.let_to_top_tac ctxt,
-   resolve_tac ctxt @{thms carry_let_eq_impI word_let_eq_impI let_eq_impI},
+fun asm_tac ctxt = full_simp_tac (put_simpset HOL_basic_ss ctxt
+        addsimps @{thms word_ineq_via_carry_val word_bit_eq_iff})
+    THEN_ALL_NEW rev_mp_prems_tac (exists_Const (fn (s, _) => s = @{const_name bit})) ctxt
+
+val is_word = can Word_Lib.dest_wordT o fastype_of
+
+fun search_term search_f t = let
+    fun sub_ts (f $ x) = [f, x]
+      | sub_ts (Abs (_, _, t)) = [t]
+      | sub_ts _ = []
+    fun f [] = NONE
+      | f (t :: ts) = case search_f t of
+        SOME x => SOME x
+      | NONE => f (sub_ts t @ ts)
+  in f [t] end
+
+fun note_let_term t = let
+    val (f, xs) = Term.strip_comb t
+    val f_nm = fst (dest_Const f)
+  in if f_nm = @{const_name carry_val} andalso is_word t
+    then SOME (t, true)
+    else if f_nm = @{const_name If} andalso is_word t andalso length xs = 3
+        andalso not (Let_Alt.is_atom (hd xs))
+    then SOME (hd xs, true)
+    else if f_nm = @{const_name Let} andalso length xs = 2
+    then SOME (hd xs, not (Let_Alt.is_atom (hd xs)))
+    else NONE
+  end handle TERM _ => NONE
+
+fun pull_let_conv ctxt ct = case search_term note_let_term (Thm.term_of ct) of
+    NONE => Conv.no_conv ct
+  | SOME (t, lift) => if lift
+    then Let_Alt.add_let_conv ctxt "x" (Thm.cterm_of ctxt t) ct
+    else Let_Alt.let_atom_conv ctxt ct
+
+fun goal_bool_conv conv ctxt = let
+    fun bool_conv ctxt ct = case Thm.term_of ct of
+        Const (@{const_name Trueprop}, _) $ _ => Conv.arg_conv (conv ctxt) ct
+      | _ => Conv.no_conv ct
+  in Conv.params_conv ~1 (fn ctxt => Conv.concl_conv ~1 (bool_conv ctxt)) ctxt end
+
+fun pull_let_step ctxt = CONVERSION (goal_bool_conv pull_let_conv ctxt)
+
+fun let_step ctxt = DETERM o FIRST'
+  [resolve_tac ctxt @{thms carry_let_eq_impI word_let_eq_impI let_eq_impI},
+   CHANGED o pull_let_step ctxt,
    CHANGED o Let_Alt.let_gather_dup_tac ctxt is_word]
 
-fun let_to_imp_tac ctxt = TRY o REPEAT_ALL_NEW (let_to_imp_step ctxt)
-
-fun let_tac ctxt = let_to_imp_tac ctxt
-    THEN_ALL_NEW rev_mp_prems_tac (exists_Const (fn (s, _) => s = @{const_name bit})) ctxt
+fun let_tac ctxt = simp_tac (put_simpset HOL_basic_ss ctxt
+        addsimps @{thms word_via_carry_val})
+    THEN_ALL_NEW (TRY o REPEAT_ALL_NEW (let_step ctxt))
 
 val len_ss = put_simpset (simpset_of \<^theory_context>\<open>Type_Length\<close>) @{context}
     |> simpset_of;
@@ -266,51 +282,53 @@ fun mk_arith_simproc ctxt = Mk_Cache_Simproc.mk ctxt "bitwise_arith_cache" len_s
   (map Logic.varify_global
     [@{term "x + y"}, @{term "x - y"},
         @{term "x < y"}, @{term "x <= y"},
+        @{term "x mod y"},
         @{term "Suc i"}, @{term "pred_numeral n"},
+        @{term "nat i"}, @{term "int n"},
         @{term "drop_bit i (n :: nat)"}, @{term "take_bit i (n :: nat)"},
         @{term "bit (i :: int) j"}, @{term "(i :: nat) = j"},
         @{term "len_of x"}])
 
 fun get_bit_simps ctxt = let
     val ss = Named_Theorems.get ctxt @{named_theorems bit_simps}
-    val _ = tracing ("get_bit_simps: length: " ^ @{make_string} (length ss))
   in ss end
 
-fun main_ss ctxt = put_simpset no_split_ss ctxt
+fun main_ss proc ctxt = put_simpset HOL_ss ctxt
+    delsimprocs [@{simproc let_simp}]
+    delsimps @{thms subst_all}
     addsimps @{thms Word.exp_eq_zero_iff one_neq_zero
         upt_conv_Cons numeral_2_eq_2[symmetric]
         upt_conv_Nil[OF order_refl]
-        list.set ball_insert ball_empty
+        ball_set_simps
         nat.case case_nat_numeral[unfolded Let_def]
         bit_word_numeral_eq_int
-        bit_if}
+        o_apply}
     addsimps (get_bit_simps ctxt)
-    addsimprocs [mk_arith_simproc ctxt]
+    addsimprocs [proc]
+    |> Splitter.del_split @{thm if_split}
 
-fun main_tac ctxt =
+fun main_tac ctxt = let
+    val proc = mk_arith_simproc ctxt
+  in
     simp_tac (put_simpset HOL_basic_ss ctxt addsimps @{thms imp_to_id word_bit_eq_iff})
-    THEN_ALL_NEW simp_tac (main_ss ctxt)
+    THEN_ALL_NEW simp_tac (main_ss proc ctxt)
     THEN_ALL_NEW simp_tac (put_simpset HOL_basic_ss ctxt
-        addsimps @{thms id_apply simp_thms carry_simps if_simps})
+        addsimps @{thms simp_thms carry_simps if_simps
+            bit_word_impossible}
+        addsimprocs [proc])
+    THEN_ALL_NEW simp_tac (put_simpset HOL_basic_ss ctxt addsimps @{thms id_apply})
+  end
 
-fun tac ctxt = init_tac ctxt
+fun tac asm ctxt = (if asm then asm_tac ctxt else K all_tac)
     THEN_ALL_NEW let_tac ctxt
     THEN_ALL_NEW main_tac ctxt
 
-(* also pull in assumptions that can be rewritten bitwise *)
-
-fun asm ctxt = full_simp_tac (put_simpset HOL_basic_ss ctxt
-        addsimps @{thms word_ineq_via_carry_val word_bit_eq_iff})
-    THEN_ALL_NEW rev_mp_prems_tac (exists_Const (fn (s, _) => s = @{const_name bit}
-        orelse s = @{const_name carry_val})) ctxt
-
-fun asm_tac ctxt = asm ctxt THEN_ALL_NEW tac ctxt
-
-fun parse_method s ctxt = Method.SIMPLE_METHOD (
-    if s = "asm" then asm_tac ctxt 1
-    else if s = "" then tac ctxt 1
-    else error ("parse_asm_tac: expected (asm) or none: " ^ s)
-  )
+fun parse_method s ctxt = let
+    val asm = if s = "no_asm" then false
+      else if s = "asm" then true
+      else if s = "" then true
+      else error ("parse_asm_tac: expected (asm) or (no_asm) or none: " ^ s)
+  in Method.SIMPLE_METHOD (tac asm ctxt 1) end
 
 end
 \<close>
@@ -327,7 +345,6 @@ method_setup word_bitwise_eq =
 lemma (* testing *)
   fixes x :: "8 word" and y :: "6 word"
   shows "or (and (ucast x) (xor y 0)) (xor y 0) = y"
-  apply (tactic \<open>BW_Alt.init_tac @{context} 1\<close>)
   apply (tactic \<open>BW_Alt.let_tac @{context} 1\<close>)
   apply (tactic \<open>BW_Alt.main_tac @{context} 1\<close>)
   apply blast
@@ -340,13 +357,37 @@ lemma (* testing *)
   apply blast
   done
 
+lemma (* testing with carry *)
+  fixes x :: "12 word"
+  shows "or (and x 53) (and y 72) = (and y 72) + (and x 53)"
+  apply (tactic \<open>BW_Alt.let_tac @{context} 1\<close>)
+  apply (tactic \<open>BW_Alt.main_tac @{context} 1\<close>)
+  apply (clarsimp simp add: carry_def)
+  done
+
+lemma (* testing with if *)
+  fixes x :: "12 word"
+  shows "(if i = j then x else 0) = (and x (if j = i then (-1) else 0))"
+  apply (tactic \<open>BW_Alt.let_tac @{context} 1\<close>)
+  apply (tactic \<open>BW_Alt.main_tac @{context} 1\<close>)
+  apply blast
+  done
+
+lemma (* testing with let *)
+  fixes x :: "12 word"
+  shows "\<And>y :: nat. True \<longrightarrow> (let z = or x 1 in (drop_bit 1 z) = (drop_bit 1 x))"
+  apply (tactic \<open>BW_Alt.let_tac @{context} 1\<close>)
+  apply (tactic \<open>BW_Alt.main_tac @{context} 1\<close>)
+  apply simp
+  done
+
 lemma (* more ugly testing *)
   fixes val :: "30 word"
   shows "P \<Longrightarrow> bit val 23 = bit (val + incr) 23 \<Longrightarrow>
-    \<not> bit incr 23 \<Longrightarrow>
+    \<not> bit incr 23 \<Longrightarrow> Q val \<Longrightarrow>
     (ucast val AND 16777215) + (ucast incr AND 16777215) \<le> (16777215::64 word)"
-  apply (word_bitwise_eq(asm))
-  apply (intro impI; simp only: carry_def simp_thms)
+  apply (word_bitwise_eq)
+  apply (intro impI; simp add: carry_def)
   apply argo
   done
 
